src/examples/matmul/GPU.MatMul.Impure.fst
@@ -18,7 +18,7 @@ fn gpu_matrix_share_underspec
   (rows columns: nat)
   (ga : gpu_array a (rows * columns))
   (shared: erased nat{shared > 0})
-  (s: erased (Seq.Base.seq a) { Seq.length s == rows * columns })
+  (s: erased (Seq.seq a) { Seq.length s == rows * columns })
   requires gpu_pts_to_matrix #a rows columns ga 1 s
   ensures bigstar #uid 0 shared (fun _ -> gpu_pts_to_matrix #a rows columns ga shared s)
 {
@@ -32,7 +32,7 @@ fn gpu_matrix_unshare_underspec
   (rows columns: nat)
   (ga : gpu_array a (rows * columns))
   (shared: erased nat{shared > 0})
-  (s: erased (Seq.Base.seq a) { Seq.length s == rows * columns })
+  (s: erased (Seq.seq a) { Seq.length s == rows * columns })
   requires bigstar #uid 0 shared (fun _ -> gpu_pts_to_matrix #a rows columns ga shared s)
   ensures  gpu_pts_to_matrix #a rows columns ga 1 s
 {
